add

clover_mbpp/clover_mbpp50_naive.py
@@ -1,0 +1,389 @@
+import argparse
+import typing 
+import os
+import pydantic
+from typing import Dict, List
+
+
+import sglang as sgl
+from sglang import OpenAI, assistant, gen, set_default_backend, system, user
+import mbpp_dataset
+
+from equiv_tests import equiv_test_code, equiv_test_doc, equiv_test_spec
+import sys_prompts
+from utils import (
+    compile_dafny,
+    extract_body,
+    extract_code_from_llm_output,
+    extract_spec,
+    get_clover_anno_check_template,
+    get_clover_mbpp_program,
+    get_clover_components,
+    get_clover_input_sample,
+    is_dafny_verified,
+    merge_pre_and_body,
+    merge_spec_and_body,
+    no_compile_error,
+    run_dafny,
+    stream_print,
+)
+
+class Result(pydantic.BaseModel):
+    verify_success: bool
+    reconstruct_success: bool
+    code: str = ""
+    trace: typing.List = []
+
+
+class Results(pydantic.RootModel):
+    root: typing.Dict[str, Result] = {}
+
+
+@sgl.function
+def gen_doc_from_body(s, body):
+    s += system(sys_prompts.SYS_DAFNY)
+    s += user(sys_prompts.GEN_DOC_FROM_BODY + body)
+    s += assistant(gen("new_doc", max_tokens=512))
+    return s["new_doc"]
+
+
+@sgl.function
+def gen_doc_from_spec(s, spec):
+    s += system(sys_prompts.SYS_DAFNY)
+    s += user(sys_prompts.GEN_DOC_FROM_SPEC + spec)
+    s += assistant(gen("new_doc", max_tokens=512))
+    return s["new_doc"]
+
+
+@sgl.function
+def gen_body_from_doc(s, doc, head, input_sample, dafny_path, feedback_turn=3):
+    s += system(sys_prompts.SYS_DAFNY)
+    s += user(sys_prompts.GEN_BODY_FROM_DOC + doc + "\n" + head)
+    for i in range(feedback_turn):
+        with s.copy() as tmp:
+            tmp += assistant(gen("new_body", max_tokens=1024))
+            body = extract_code_from_llm_output(tmp["new_body"])
+        body = extract_body(body.strip().split("\n"), False)
+        s += assistant(body)
+        out = compile_dafny(body, dafny_path)
+        if no_compile_error(str(out)):
+            return body
+        with s.user():
+            s += "This answer got Dafny compile error:\n" + str(out) + "\n"
+            s += "Please try again by taking the Dafny compiler feedback."
+    return body
+
+
+@sgl.function
+def gen_body_from_spec(s, spec, dafny_path, feedback_turn=3):
+    s += system(sys_prompts.SYS_DAFNY)
+    s += user(sys_prompts.GEN_BODY_FROM_SPEC + spec)
+    body = ""
+    for i in range(feedback_turn):
+        with s.copy() as tmp:
+            tmp += assistant(gen("body", max_tokens=1024))
+            body = extract_code_from_llm_output(tmp["body"])
+        body = extract_body(body.strip().split("\n"), False)
+        s += assistant(body)
+        out = compile_dafny(body, dafny_path)
+        if no_compile_error(str(out)):
+            return True, body
+        with s.user():
+            s += "This answer got Dafny compile error:\n" + str(out) + "\n"
+            s += "Please try again by taking the Dafny compiler feedback."
+
+    return False, body
+
+
+@sgl.function
+def gen_spec_from_doc(s, doc, head, dafny_path, feedback_turn=3):
+    s += system(sys_prompts.SYS_DAFNY)
+    s += user(sys_prompts.GEN_SPEC_FROM_DOC + doc + "\n" + head)
+    for i in range(feedback_turn):
+        with s.copy() as tmp:
+            tmp += assistant(gen("new_spec", max_tokens=512))
+            spec = extract_code_from_llm_output(tmp["new_spec"])
+        spec = extract_spec(spec.strip().split("\n"), False)
+        s += assistant(spec)
+
+        out = compile_dafny(spec, dafny_path)
+        if no_compile_error(str(out)):
+            return spec
+        with s.user():
+            s += "This answer got Dafny compile error:\n" + str(out) + "\n"
+            s += "Please try again by taking the Dafny compiler feedback."
+
+    return spec
+
+
+def doc_to_body_reconstruct(
+    doc: str, body: str, input_sample: str, dafny_path, feedback_turn=3, num_trial=1, verbose=0
+):
+    head = body.split("\n")[0]
+    success = False
+    for k in range(num_trial):
+        s = gen_body_from_doc(
+            doc, head, input_sample, dafny_path, feedback_turn=feedback_turn, stream=(
+                verbose >= 2)
+        )
+        if verbose >= 2:
+            stream_print(s)
+        new_body = str(s.ret_value)
+        if not equiv_test_code(body, new_body, input_sample, dafny_path, verbose=verbose):
+            if verbose >= 2:
+                print(
+                    f"\n###### Clover Info::Attempt ({k+1}) Doc -> body reconstruction failed.\n"
+                )
+        else:
+            if verbose >= 1:
+                print(
+                    f"\n###### Clover Info::Attempt ({k+1}) Doc -> body reconstruction succeeded.\n"
+                )
+            success = True
+            break
+    if not success and verbose >= 1:
+        print(
+            f"\n###### Clover Info::Doc -> body reconstruction failed for {num_trial} attempts.\n"
+        )
+    return success
+
+
+def body_to_doc_reconstruct(doc: str, body: str, num_trial=1, verbose=0):
+    head = body.split("\n")[0]
+    success = False
+    for k in range(num_trial):
+        s = gen_doc_from_body(body, stream=(verbose >= 2))
+        if verbose >= 2:
+            stream_print(s)
+        new_doc = str(s.ret_value)
+        if not equiv_test_doc(doc, new_doc, head, verbose=verbose):
+            if verbose >= 2:
+                print(
+                    f"\n###### Clover Info::Attempt ({k+1}) Body -> doc reconstruction failed.\n"
+                )
+        else:
+            if verbose >= 1:
+                print(
+                    f"\n###### Clover Info::Attempt ({k+1}) Body -> doc reconstruction succeeded.\n"
+                )
+            success = True
+            break
+    if not success and verbose >= 1:
+        print(
+            f"\n###### Clover Info::Body -> doc reconstruction failed for {num_trial} attempts.\n"
+        )
+    return success
+
+
+def doc_to_spec_reconstruct(
+    doc: str, spec: str, anno_check_template: Dict[str, str], dafny_path, num_trial=1, verbose=0
+):
+    head = spec.split("\n")[0]
+    success = False
+    for k in range(num_trial):
+        s = gen_spec_from_doc(doc, head, dafny_path, stream=(verbose >= 2))
+        if verbose >= 2:
+            stream_print(s)
+        new_spec = str(s.ret_value)
+        if not equiv_test_spec(spec, new_spec, anno_check_template, dafny_path, verbose=verbose):
+            if verbose >= 2:
+                print(
+                    f"\n###### Clover Info::Attempt ({k+1}) Doc -> spec reconstruction failed.\n"
+                )
+
+        else:
+            if verbose >= 1:
+                print(
+                    f"\n###### Clover Info::Attempt ({k+1}) Doc -> spec reconstruction succeeded.\n"
+                )
+            success = True
+            break
+    if not success and verbose >= 1:
+        print(
+            f"\n###### Clover Info::Doc -> spec reconstruction failed for {num_trial} attempts.\n"
+        )
+    return success
+
+
+def spec_to_doc_reconstruct(doc: str, spec: str, num_trial=1, verbose=0):
+    head = spec.split("\n")[0]
+    success = False
+    for k in range(num_trial):
+        s = gen_doc_from_spec(spec, stream=(verbose >= 2))
+        if verbose >= 2:
+            stream_print(s)
+        new_doc = str(s.ret_value)
+        if not equiv_test_doc(doc, new_doc, head, verbose=verbose):
+            if verbose >= 2:
+                print(
+                    f"\n###### Clover Info::Attempt ({k+1}) Spec -> doc reconstruction failed.\n"
+                )
+        else:
+            if verbose >= 1:
+                print(
+                    f"\n###### Clover Info::Attempt ({k+1}) Spec -> doc reconstruction succeeded.\n"
+                )
+            success = True
+            break
+    if not success and verbose >= 1:
+        print(
+            f"\n###### Clover Info::Spec -> doc reconstruction failed for {num_trial} attempts.\n"
+        )
+    return success
+
+
+def spec_soundness(spec: str, body: str, dafny_path, verbose=0):
+    body_with_spec = merge_spec_and_body(spec, body)
+    out, err = run_dafny(body_with_spec, dafny_path)
+    if not is_dafny_verified(str(out)):
+        if verbose >= 1:
+            print("\n###### Clover Info::Dafny verifier failed.\n")
+        return False
+    if verbose >= 1:
+        print("\n###### Clover Info::Dafny verifier passed.\n")
+    return True
+
+
+def spec_to_body_reconstruct(
+    spec: str, body: str, input_sample: str, dafny_path, feedback_turn=3, num_trial=1, verbose=0
+):
+    # completeness (spec -> body)
+    success = False
+    for k in range(num_trial):
+        s = gen_body_from_spec(
+            spec, dafny_path, feedback_turn=feedback_turn, stream=(verbose >= 2))
+        if verbose >= 2:
+            stream_print(s)
+        verified, new_body = s.ret_value
+        if not verified:
+            if verbose >= 2:
+                print(
+                    f"\n###### Clover Info::Attempt ({k+1}) Failed to reconstruct a body that can be verified.\n"
+                )
+        elif not equiv_test_code(body, new_body, input_sample, dafny_path, verbose=verbose):
+            if verbose >= 2:
+                print(
+                    f"\n###### Clover Info::Attempt ({k+1}) Spec -> body reconstruction failed.\n"
+                )
+        else:
+            if verbose >= 1:
+                print(
+                    f"\n###### Clover Info::Attempt ({k+1}) Spec -> body reconstruction succeeded.\n"
+                )
+            success = True
+            break
+    if not success and verbose >= 1:
+        print(
+            f"\n###### Clover Info::Spec -> body reconstruction failed for {num_trial} attempts.\n"
+        )
+    return success
+
+
+def clover(
+    program: List[str],
+    input_sample,
+    anno_check_template,
+    dafny_path,
+    feedback_turn=3,
+    num_trial=1,
+    verbose=0,
+    early_quit=False,
+):
+    doc, spec, body = get_clover_components(program)
+    ret = [None] * 6
+    # doc & body consistency
+    ret[0] = doc_to_body_reconstruct(
+        doc,
+        body,
+        input_sample,
+        dafny_path,
+        feedback_turn=feedback_turn,
+        num_trial=num_trial,
+        verbose=verbose,
+    )
+    if early_quit and not ret[0]:
+        return False, ret
+    body_with_pre = merge_pre_and_body(spec, body)
+    ret[1] = body_to_doc_reconstruct(
+        doc, body_with_pre, num_trial=num_trial, verbose=verbose
+    )
+    if early_quit and not ret[1]:
+        return False, ret
+
+    # doc & spec consistency
+    ret[2] = doc_to_spec_reconstruct(
+        doc, spec, anno_check_template, dafny_path, num_trial=num_trial, verbose=verbose
+    )
+    if early_quit and not ret[2]:
+        return False, ret
+    ret[3] = spec_to_doc_reconstruct(
+        doc, spec, num_trial=num_trial, verbose=verbose)
+    if early_quit and not ret[3]:
+        return False, ret
+
+    # spec & body consistency
+    ret[4] = spec_soundness(spec, body, dafny_path, verbose=verbose)
+    if early_quit and not ret[4]:
+        return False, ret
+    ret[5] = spec_to_body_reconstruct(
+        spec,
+        body,
+        input_sample,
+        dafny_path,
+        feedback_turn=feedback_turn,
+        num_trial=num_trial,
+        verbose=verbose,
+    )
+    if early_quit and not ret[5]:
+        return False, ret
+    if verbose >= 2:
+        print("\n###### Final Clover Result: ", all(ret), ret)
+
+    return all(ret), ret
+
+
+
+
+if __name__ == "__main__":
+    parser = argparse.ArgumentParser()
+    parser.add_argument("--test-name", type=str, default="task_id_58")
+    parser.add_argument("--verbose", type=int, default=3)
+    parser.add_argument("--early-quit", action="store_true")
+    parser.add_argument("--dafny-path", type=str, default="dafny")
+    parser.add_argument("--feedback-turn", type=int, default=3)
+    parser.add_argument("--num-trial", type=int, default=1)
+    args = parser.parse_args()
+
+    result_path = "clover_mbpp_naive_results.json"
+
+    # backend = OpenAI("gpt-3.5-turbo")
+    # backend = OpenAI("gpt-4")
+    set_default_backend(OpenAI("gpt-4-1106-preview"))
+    # set_default_backend(OpenAI("gpt-4"))
+
+    program_path = (
+        f"../dataset/MBPP-DFY-50/src/{args.test_name}.dfy"
+    )
+    program_with_pre_path = f"../dataset/MBPP-DFY-50/{args.test_name}.dfy"
+    doc_path = (
+        f"../dataset/MBPP-DFY-50/mbpp-dfy-50-examples-db.json"
+    )
+    task_id=args.test_name.split("_")[-1]
+    input_sample_path = f"../dataset/MBPP-DFY-50/test/{args.test_name}.dfy"
+    anno_check_template_path = f"../dataset/MBPP-DFY-50/anno_template/{args.test_name}.dfy"
+
+    program = get_clover_mbpp_program(program_path, doc_path, task_id)
+    input_sample = get_clover_input_sample(input_sample_path)
+    anno_check_template = get_clover_anno_check_template(
+        anno_check_template_path)
+    print(
+        "Passed the Clover test?",
+        clover(
+            program,
+            input_sample,
+            anno_check_template,
+            args.dafny_path,
+            verbose=args.verbose,
+            early_quit=args.early_quit,
+        ),
+    )
