dataset/MBPP-DFY-50/anno_template/task_id_588.dfy
@@ -1,0 +1,37 @@
+predicate pre_original(a: array<int>, diff: int)
+reads a
+{
+true
+}
+
+predicate pre_gen(a: array<int>, diff: int)
+reads a
+{
+  true // (#PRE) && ... (#PRE)
+}
+
+lemma pre_eq(a: array<int>, diff: int)
+  ensures pre_original(a, diff) <==> pre_gen(a, diff)
+{
+}
+
+predicate post_original(a: array<int>, diff: int)
+  requires pre_original(a, diff)
+  reads a
+{
+true
+}
+
+predicate post_gen(a: array<int>, diff: int)
+  requires pre_original(a, diff)
+  reads a
+{
+  true // (#POST) && ... (#POST)
+}
+
+lemma post_eq(a: array<int>, diff: int)
+  requires pre_original(a, diff)
+  requires pre_gen(a, diff)
+  ensures post_original(a, diff) <==> post_gen(a, diff)
+{
+}
