dataset/MBPP-DFY-50/anno_template/task_id_632.dfy
@@ -1,0 +1,37 @@
+predicate pre_original(arr: array<int>)
+reads arr
+{
+true
+}
+
+predicate pre_gen(arr: array<int>)
+reads arr
+{
+  true // (#PRE) && ... (#PRE)
+}
+
+lemma pre_eq(arr: array<int>)
+  ensures pre_original(arr) <==> pre_gen(arr)
+{
+}
+
+predicate post_original(arr: array<int>)
+  requires pre_original(arr)
+  reads arr
+{
+true
+}
+
+predicate post_gen(arr: array<int>)
+  requires pre_original(arr)
+  reads arr
+{
+  true // (#POST) && ... (#POST)
+}
+
+lemma post_eq(arr: array<int>)
+  requires pre_original(arr)
+  requires pre_gen(arr)
+  ensures post_original(arr) <==> post_gen(arr)
+{
+}
