dataset/MBPP-DFY-50/src/task_id_477.dfy
@@ -1,18 +1,3 @@
-predicate IsUpperCase(c : char)
-{
-  65 <= c as int <= 90
-}
-
-predicate IsUpperLowerPair(C : char, c : char)
-{
-  (C as int) == (c as int) - 32
-}
-
-function Shift32(c : char) :  char
-{
-  ((c as int + 32) % 128) as char
-}
-
 method ToLowercase(s: string) returns (v: string)
   ensures |v| == |s|
   ensures forall i :: 0 <= i < |s| ==>  if IsUpperCase(s[i]) then IsUpperLowerPair(s[i], v[i]) else v[i] == s[i]
@@ -35,3 +20,19 @@ method ToLowercase(s: string) returns (v: string)
   }
   return s';
 }
+
+predicate IsUpperCase(c : char)
+{
+  65 <= c as int <= 90
+}
+
+predicate IsUpperLowerPair(C : char, c : char)
+{
+  (C as int) == (c as int) - 32
+}
+
+function Shift32(c : char) :  char
+{
+  ((c as int + 32) % 128) as char
+}
+
