dataset/MBPP-DFY-50/src/task_id_632.dfy
@@ -3,7 +3,7 @@ method MoveZeroesToEnd(arr: array<int>)
   modifies arr
   ensures forall i, j :: 0 <= i < j < arr.Length && arr[i] == 0 ==> arr[j] == 0
   ensures multiset(arr[..]) == multiset(old(arr[..]))
-  ensures forall n, m /* on old array */:: 0 <= n < m < arr.Length && old(arr[n]) != 0 && old(arr[m]) != 0 ==>
+  ensures forall n, m :: 0 <= n < m < arr.Length && old(arr[n]) != 0 && old(arr[m]) != 0 ==>
                                              exists k, l /* on new array */:: 0 <= k < l < arr.Length && arr[k] == old(arr[n]) && arr[l] == old(arr[m])
   
 {
