dataset/MBPP-DFY-50/src/task_id_775.dfy
@@ -1,8 +1,3 @@
-predicate IsOdd(n: int)
-{
-  n % 2 == 1
-}
-
 method IsOddAtIndexOdd(a: array<int>) returns (result: bool)
   ensures result <==> forall i :: 0 <= i < a.Length ==> (IsOdd(i) ==> IsOdd(a[i]))
 {
@@ -18,3 +13,9 @@ method IsOddAtIndexOdd(a: array<int>) returns (result: bool)
     }
   }
 }
+
+predicate IsOdd(n: int)
+{
+  n % 2 == 1
+}
+
