dataset/MBPP-DFY-50/src/task_id_784.dfy
@@ -1,27 +1,13 @@
-predicate IsEven(n: int)
+method ProductEvenOdd(lst: seq<int>) returns (product : int)
+  requires |lst| >= 2
+  requires exists i :: 0 <= i < |lst| && IsEven(lst[i])
+  requires exists i :: 0 <= i < |lst| && IsOdd(lst[i])
+  ensures exists i, j :: 0 <= i < |lst| && IsEven(lst[i]) && IsFirstEven(i, lst) &&
+                         0 <= j < |lst| && IsOdd(lst[j])  && IsFirstOdd(j, lst) && product == lst[i] * lst[j]
 {
-  n % 2 == 0
+  var evenIndex, oddIndex := FirstEvenOddIndices(lst);
+  product := lst[evenIndex] * lst[oddIndex];
 }
-
-predicate IsOdd(n: int)
-{
-  n % 2 != 0
-}
-
-predicate IsFirstEven(evenIndex: int, lst: seq<int>)
-  requires 0 <= evenIndex < |lst|
-  requires IsEven(lst[evenIndex])
-{
-  forall i :: 0 <= i < evenIndex ==> IsOdd(lst[i])
-}
-
-predicate IsFirstOdd(oddIndex: int, lst: seq<int>)
-  requires 0 <= oddIndex < |lst|
-  requires IsOdd(lst[oddIndex])
-{
-  forall i :: 0 <= i < oddIndex ==> IsEven(lst[i])
-}
-
 
 method FirstEvenOddIndices(lst : seq<int>) returns (evenIndex: int, oddIndex : int)
   requires |lst| >= 2
@@ -55,13 +41,30 @@ method FirstEvenOddIndices(lst : seq<int>) returns (evenIndex: int, oddIndex : i
   }
 }
 
-method ProductEvenOdd(lst: seq<int>) returns (product : int)
-  requires |lst| >= 2
-  requires exists i :: 0 <= i < |lst| && IsEven(lst[i])
-  requires exists i :: 0 <= i < |lst| && IsOdd(lst[i])
-  ensures exists i, j :: 0 <= i < |lst| && IsEven(lst[i]) && IsFirstEven(i, lst) &&
-                         0 <= j < |lst| && IsOdd(lst[j])  && IsFirstOdd(j, lst) && product == lst[i] * lst[j]
+
+
+predicate IsEven(n: int)
 {
-  var evenIndex, oddIndex := FirstEvenOddIndices(lst);
-  product := lst[evenIndex] * lst[oddIndex];
+  n % 2 == 0
 }
+
+predicate IsOdd(n: int)
+{
+  n % 2 != 0
+}
+
+predicate IsFirstEven(evenIndex: int, lst: seq<int>)
+  requires 0 <= evenIndex < |lst|
+  requires IsEven(lst[evenIndex])
+{
+  forall i :: 0 <= i < evenIndex ==> IsOdd(lst[i])
+}
+
+predicate IsFirstOdd(oddIndex: int, lst: seq<int>)
+  requires 0 <= oddIndex < |lst|
+  requires IsOdd(lst[oddIndex])
+{
+  forall i :: 0 <= i < oddIndex ==> IsEven(lst[i])
+}
+
+
